fairis/heap_lang/examples/yesno/yesno_mus.v
@@ -9,20 +9,7 @@ From trillium.program_logic Require Export weakestpre.
 From trillium.fairness Require Import fairness fair_termination fuel sswp_rules resources action_model utils.
 From trillium.fairness.heap_lang Require Export lang lifting tactics proofmode notation iris_inst.
 From trillium.fairness.heap_lang.examples Require Import env_am split_model mu_role.
-From trillium.fairness.heap_lang.examples.yesno Require Import yesno_model.
-
-
-(** The CMRAs we need. *)
-Class yesnoG Σ := YesnoG {
-  yes_name: gname;
-  no_name: gname;
-  yesno_n_G :> inG Σ (excl_authR natO);
-  yesno_f_G :> inG Σ (excl_authR boolO);
- }.
-Class yesnoPreG Σ := {
-  yesno_PreG :> inG Σ (excl_authR natO);
-  yesno_f_PreG :> inG Σ (excl_authR boolO);
- }.
+From trillium.fairness.heap_lang.examples.yesno Require Import yesno_model yesno_threads.
 
 
 Section FullModel.
@@ -57,51 +44,11 @@ Section MUs.
 
   Let Ns := nroot .@ "yes_no".
 
-  Definition yes_at (n: nat) := own yes_name (◯E n).
-  Definition no_at (n: nat) := own no_name (◯E n).
-
-  Definition auth_yes_at (n: nat) := own yes_name (●E n).
-  Definition auth_no_at (n: nat) := own no_name (●E n).
-
-  Lemma they_agree γ (n m: nat) :
-    own γ (◯E n) -∗ own γ (●E m) -∗ ⌜ m = n ⌝.
-  Proof.
-    iIntros "HA HB". iCombine "HB HA" as "H".
-    iDestruct (own_valid with "H") as "%Hval".
-    iPureIntro. by apply excl_auth_agree_L.
-  Qed.
-  Lemma yes_agree n m :
-    yes_at n -∗ auth_yes_at m -∗ ⌜ m = n ⌝.
-  Proof. apply they_agree. Qed.
-  Lemma no_agree n m :
-    no_at n -∗ auth_no_at m -∗ ⌜ m = n ⌝.
-  Proof. apply they_agree. Qed.
-
-  Lemma they_update γ (n m P: nat) :
-    own γ (●E n) ∗ own γ (◯E m) ==∗ own γ (●E P) ∗ own γ (◯E P).
-  Proof.
-    rewrite -!own_op. iApply own_update. apply excl_auth_update.
-  Qed.
-  Lemma yes_update P n m :
-     auth_yes_at m ∗ yes_at n ==∗ auth_yes_at P ∗ yes_at P.
-  Proof. apply they_update. Qed.
-  Lemma no_update P n m :
-     auth_no_at m ∗ no_at n ==∗ auth_no_at P ∗ no_at P.
-  Proof. apply they_update. Qed.
-
   Lemma they_finished_update γ (n m P: bool) :
     own γ (●E n) ∗ own γ (◯E m) ==∗ own γ (●E P) ∗ own γ (◯E P).
   Proof.
     rewrite -!own_op. iApply own_update. apply excl_auth_update.
   Qed.
-
-  Definition yn_corr l n b: iProp Σ := 
-      (⌜(n, b) ≠ (0, false)⌝ ∗
-      (* frag_right_st_is (n, b) ∗ *)
-      l ↦ #b ∗
-      if b
-      then auth_yes_at n ∗ auth_no_at n
-      else auth_yes_at (n-1) ∗ auth_no_at n)%I.
 
   Definition yesno_inv_inner b : iProp Σ :=
     ∃ n B,
@@ -110,24 +57,12 @@ Section MUs.
 
   Let yn_role (ρ: YN): amRole PM := inr ρ.
 
-  Definition yes_vs l ι: iProp Σ :=
-    □ |={⊤, ⊤ ∖ ↑ι}=> ∃ n b,
-      (▷ yn_corr l n b) ∗
-      ((⌜ if b then n > 0 else n > 1 ⌝ -∗ MU__r (yn_role Y) (⊤ ∖ ↑ι)
-         (* redundancy to ease subsequent adaptation for No thread *)
-           (▷ (if b then yn_corr l n false else yn_corr l n false) ={⊤ ∖ ↑ι, ⊤}=∗ True)
-       ) ∧
-       (⌜ n = 0 /\ b = true \/ n = 1 /\ b = false ⌝ -∗ 
-        MU__drop (yn_role Y) (⊤ ∖ ↑ι) (▷ yn_corr l n b ={⊤ ∖ ↑ι, ⊤}=∗ True))
-      ).
-
   Lemma mu_yes n (b: bool) (ns: namespace)
     (NB: if b then n > 0 else n > 1):
     inv ns (split_inv_inner) ⊢ frag_right_st_is (n, b) -∗ 
       MU__r (yn_role Y) (↑ ns) (frag_right_st_is $ if b then (n, false) else (n, false)).
   Proof using INDEP.
     rewrite /MU__r. iIntros "#INV ST" (tid f' R) "[MAP %DISJ__R]".
-    (* destruct st as [[st__e st__o] st__env]. *)
 
     enough (exists a, amTrans yn_AM (n, b) (a, Some Y) (if b then (n, false) else (n, false))) as (a & TRANS). 
     { iApply (MU_inv with "[$]"); [done| ].
@@ -154,6 +89,42 @@ Section MUs.
     exists yn_act. simpl. destruct b; by constructor. 
   Qed.
 
+  Lemma mu_no n (b: bool) (ns: namespace)
+    (NB: if b then n > 0 else n > 0)
+    :
+    inv ns (split_inv_inner) ⊢ frag_right_st_is (n, b) -∗ 
+      MU__r (yn_role No) (↑ ns) (frag_right_st_is $ if b then (n, true) else (n - 1, true)).
+  Proof using INDEP.
+    rewrite /MU__r. iIntros "#INV ST" (tid f' R) "[MAP %DISJ__R]".
+
+    enough (exists a, amTrans yn_AM (n, b) (a, Some No) (if b then (n, true) else (n - 1, true))) as (a & TRANS). 
+    { iApply (MU_inv with "[$]"); [done| ].
+      (* TODO: avoid unfolding of MU *)
+      rewrite /split_inv_inner. simpl. iIntros ">(%S & FRAG & PROD)". destruct S.
+      simpl. iDestruct (right_agree with "[$] [$]") as %->.
+
+      iMod (update_right ((if b then (n, true) else (n - 1, true)): amSt yn_AM) with "[$] [$]") as "[PROD ST]".
+      iApply (MU_wand with "[ST PROD]").
+      2: { iApply (model_step_MU with "[$] [MAP]").
+           1, 4: by eauto.
+           { simpl. eapply am_fmtrans_action. eexists. 
+             eapply pt_inner2; eauto.
+             intros ?. edestruct INDEP; eauto.
+             eapply action_of_step; eauto. }
+           simpl. setoid_rewrite @prod_indep_live_roles; eauto.
+           apply union_mono; [done| ]. apply set_map_mono; [done| ].
+           erewrite !yn_AM_live_roles'.
+           simpl. destruct b, n as [|[|]]; simpl; try set_solver.
+           destruct n; done. }
+      iIntros "(MAP & FRAG)".
+      iFrame. }
+    Unshelve. 2: by apply _.
+
+    assert (n > 0) by (by destruct b). destruct n; [lia| ].
+    simpl. rewrite Nat.sub_0_r. 
+    exists yn_act. simpl. destruct b; by constructor. 
+  Qed.
+
   Lemma dealloc_yes n (b: bool) (ns: namespace)
     (NB: n = 0 /\ b = true \/ n = 1 /\ b = false):
     inv ns (split_inv_inner) ⊢ frag_right_st_is (n, b) -∗
@@ -166,9 +137,6 @@ Section MUs.
     iApply fupd_pre_step. iMod "FRAG". iMod "PROD". iModIntro. 
     simpl. iDestruct (right_agree with "[$] [$]") as %->.
 
-    (* iApply (pre_step_mono with "[ST MAP]"). *)
-    (* 2: { iApply (has_fuels_dealloc with "[$]").  *)
-    
     iMod (has_fuels_dealloc _ _ _ (yn_role Y: fmrole M) with "FRAG MAP") as "[FRAG MAP]".
     { simpl. rewrite prod_indep_live_roles. apply not_elem_of_union.
       split; [set_solver| ].
@@ -181,12 +149,36 @@ Section MUs.
     by iFrame.
   Qed. 
 
+  Lemma dealloc_no n (b: bool) (ns: namespace)
+    (NB: n = 0):
+    inv ns (split_inv_inner) ⊢ frag_right_st_is (n, b) -∗
+        MU__drop (yn_role No) (↑ ns) (frag_right_st_is (n, b)). 
+  Proof using INDEP. 
+    rewrite /MU__drop. iIntros "#INV ST" (tid f' R) "[MAP %DISJ__R]".
+
+    iApply (pre_step_inv with "[$]"); [done| ].
+    rewrite /split_inv_inner. simpl. iIntros "(%S & FRAG & PROD)". destruct S.
+    iApply fupd_pre_step. iMod "FRAG". iMod "PROD". iModIntro. 
+    simpl. iDestruct (right_agree with "[$] [$]") as %->.
+
+    iMod (has_fuels_dealloc _ _ _ (yn_role No: fmrole M) with "FRAG MAP") as "[FRAG MAP]".
+    { simpl. rewrite prod_indep_live_roles. apply not_elem_of_union.
+      split; [set_solver| ].
+      intros IN%elem_of_map_inj_gset; [| by apply _].
+      rewrite yn_AM_live_roles in IN.
+      subst. destruct b; set_solver. }
+
+    iModIntro. rewrite -insert_union_singleton_l delete_insert_dom.
+    2: set_solver.
+    by iFrame.
+  Qed. 
+
   Definition yesno_inv b := inv Ns (yesno_inv_inner b).
 
   Definition Ns__split := nroot .@ "split".
 
   Lemma yes_vs_from_invs l:
-    yesno_inv l ∗ split_inv Ns__split  ⊢ yes_vs l Ns.
+    yesno_inv l ∗ split_inv Ns__split  ⊢ yes_vs l Ns (yn_role Y).
   Proof using INDEP.
     rewrite /yes_vs. iIntros "#[INV1 INV2]". iModIntro.
     iMod (inv_acc with "INV1") as "[OPEN CLOS]".
@@ -215,6 +207,41 @@ Section MUs.
       { assert (Ns__split ## Ns) by solve_ndisj. set_solver. }
       iApply (MU__drop_wand with "[-RIGHT]"). 
       2: { by iApply (dealloc_yes with "[$]"). }
+      iIntros "RIGHT CORR".
+      iMod ("CLOS" with "[-]"); [| done].
+      rewrite /yesno_inv_inner. iNext.
+      iFrame. 
+  Qed.
+
+  Lemma no_vs_from_invs l:
+    yesno_inv l ∗ split_inv Ns__split  ⊢ no_vs l Ns (yn_role No).
+  Proof using INDEP.
+    rewrite /no_vs. iIntros "#[INV1 INV2]". iModIntro.
+    iMod (inv_acc with "INV1") as "[OPEN CLOS]".
+    { apply top_subseteq. }
+    
+    rewrite {1}/yesno_inv_inner. rewrite {1}/yn_corr.  
+    iDestruct "OPEN" as (n b) "((>%NEQ & >LOC & AUTHS) & >RIGHT)".
+    iModIntro.
+    iExists _, _. iSplitL "LOC AUTHS".
+    { by iFrame. }
+
+    iSplit. 
+    - iIntros "%B". 
+      iApply (MU__r_mask_weaken (↑ Ns__split) with "[-]").
+      { assert (Ns__split ## Ns) by solve_ndisj. set_solver. }
+      iApply (MU__r_wand with "[-RIGHT]").
+      2: { by iApply (mu_no with "[$] [$]"). }
+      iIntros "RIGHT CORR".
+      iMod ("CLOS" with "[-]"); [| done].
+      rewrite /yesno_inv_inner. iNext.
+      iExists (if b then n else n - 1), true.
+      destruct b; iFrame.
+    - iIntros "%NB". 
+      iApply (MU__drop_mask_weaken (↑ Ns__split) with "[-]").
+      { assert (Ns__split ## Ns) by solve_ndisj. set_solver. }
+      iApply (MU__drop_wand with "[-RIGHT]"). 
+      2: { by iApply (dealloc_no with "[$]"). }
       iIntros "RIGHT CORR".
       iMod ("CLOS" with "[-]"); [| done].
       rewrite /yesno_inv_inner. iNext.
