fairis/heap_lang/examples/yesno/yesno_threads.v
@@ -1,0 +1,96 @@
+From stdpp Require Import decidable.
+From iris.prelude Require Import options.
+From iris.algebra Require Import excl_auth.
+From iris.bi Require Import bi.
+From iris.base_logic.lib Require Import invariants.
+From iris.proofmode Require Import tactics.
+From trillium.prelude Require Export finitary quantifiers sigma classical_instances.
+From trillium.program_logic Require Export weakestpre.
+From trillium.fairness Require Import fairness utils action_model resources fuel.
+From trillium.fairness.heap_lang Require Export lang lifting tactics proofmode.
+From trillium.fairness.heap_lang Require Import notation iris_inst lifting sswp_rules.
+From trillium.fairness.heap_lang.examples Require Import mu_role.
+Close Scope Z. 
+
+
+(** The CMRAs we need. *)
+Class yesnoG Σ := YesnoG {
+  yes_name: gname;
+  no_name: gname;
+  yesno_n_G :> inG Σ (excl_authR natO);
+  yesno_f_G :> inG Σ (excl_authR boolO);
+ }.
+Class yesnoPreG Σ := {
+  yesno_PreG :> inG Σ (excl_authR natO);
+  yesno_f_PreG :> inG Σ (excl_authR boolO);
+ }.
+
+
+Section Threads.
+  Context `{LM: LiveModel heap_lang M}.
+  Context `{!heapGS Σ LM}.
+  Context `{yesnoG Σ}. 
+  
+  Definition yes_at (n: nat) := own yes_name (◯E n).
+  Definition no_at (n: nat) := own no_name (◯E n).
+
+  Definition auth_yes_at (n: nat) := own yes_name (●E n).
+  Definition auth_no_at (n: nat) := own no_name (●E n).
+
+  Lemma they_agree γ (n m: nat) :
+    own γ (◯E n) -∗ own γ (●E m) -∗ ⌜ m = n ⌝.
+  Proof.
+    iIntros "HA HB". iCombine "HB HA" as "H".
+    iDestruct (own_valid with "H") as "%Hval".
+    iPureIntro. by apply excl_auth_agree_L.
+  Qed.
+  Lemma yes_agree n m :
+    yes_at n -∗ auth_yes_at m -∗ ⌜ m = n ⌝.
+  Proof. apply they_agree. Qed.
+  Lemma no_agree n m :
+    no_at n -∗ auth_no_at m -∗ ⌜ m = n ⌝.
+  Proof. apply they_agree. Qed.
+
+  Lemma they_update γ (n m P: nat) :
+    own γ (●E n) ∗ own γ (◯E m) ==∗ own γ (●E P) ∗ own γ (◯E P).
+  Proof.
+    rewrite -!own_op. iApply own_update. apply excl_auth_update.
+  Qed.
+  Lemma yes_update P n m :
+     auth_yes_at m ∗ yes_at n ==∗ auth_yes_at P ∗ yes_at P.
+  Proof. apply they_update. Qed.
+  Lemma no_update P n m :
+     auth_no_at m ∗ no_at n ==∗ auth_no_at P ∗ no_at P.
+  Proof. apply they_update. Qed.
+
+  Definition yn_corr l n b: iProp Σ := 
+      (⌜(n, b) ≠ (0, false)⌝ ∗
+      (* frag_right_st_is (n, b) ∗ *)
+      l ↦ #b ∗
+      if b
+      then auth_yes_at n ∗ auth_no_at n
+      else auth_yes_at (n-1) ∗ auth_no_at n)%I.
+
+  Definition yes_vs l ι (ρ: fmrole M): iProp Σ :=
+    □ |={⊤, ⊤ ∖ ↑ι}=> ∃ n b,
+      (▷ yn_corr l n b) ∗
+      ((⌜ if b then n > 0 else n > 1 ⌝ -∗ MU__r ρ (⊤ ∖ ↑ι)
+         (* redundancy to ease subsequent adaptation for No thread *)
+           (▷ (if b then yn_corr l n false else yn_corr l n false) ={⊤ ∖ ↑ι, ⊤}=∗ True)
+       ) ∧
+       (⌜ n = 0 /\ b = true \/ n = 1 /\ b = false ⌝ -∗ 
+        MU__drop ρ (⊤ ∖ ↑ι) (▷ yn_corr l n b ={⊤ ∖ ↑ι, ⊤}=∗ True))
+      ).
+
+  Definition no_vs l ι (ρ: fmrole M): iProp Σ :=
+    □ |={⊤, ⊤ ∖ ↑ι}=> ∃ n b,
+      (▷ yn_corr l n b) ∗
+      ((⌜ if b then n > 0 else n > 0 ⌝ -∗ MU__r ρ (⊤ ∖ ↑ι)
+           (▷ (if b then yn_corr l n true else yn_corr l (n - 1) true) ={⊤ ∖ ↑ι, ⊤}=∗ True)
+       ) ∧
+       (
+         ⌜ n = 0 ⌝ -∗
+        MU__drop ρ (⊤ ∖ ↑ι) (▷ yn_corr l n b ={⊤ ∖ ↑ι, ⊤}=∗ True))
+      ).
+
+End Threads.
